\left(\begin{array}{ccc} \left(y^2+z^2\right)\,\left(\cos\left(\mathrm{theta}\right)-1\right)+1=\frac{109}{125} & z\,\sin\left(\mathrm{theta}\right)-x\,y\,\left(\cos\left(\mathrm{theta}\right)-1\right)=-\frac{12}{25} & y\,\sin\left(\mathrm{theta}\right)+x\,z\,\left(\cos\left(\mathrm{theta}\right)-1\right)=\frac{12}{125}\\ -z\,\sin\left(\mathrm{theta}\right)-x\,y\,\left(\cos\left(\mathrm{theta}\right)-1\right)=\frac{12}{25} & \left(x^2+z^2\right)\,\left(\cos\left(\mathrm{theta}\right)-1\right)+1=\frac{4}{5} & y\,z\,\left(\cos\left(\mathrm{theta}\right)-1\right)-x\,\sin\left(\mathrm{theta}\right)=-\frac{9}{25}\\ x\,z\,\left(\cos\left(\mathrm{theta}\right)-1\right)-y\,\sin\left(\mathrm{theta}\right)=\frac{12}{125} & x\,\sin\left(\mathrm{theta}\right)+y\,z\,\left(\cos\left(\mathrm{theta}\right)-1\right)=\frac{9}{25} & \left(x^2+y^2\right)\,\left(\cos\left(\mathrm{theta}\right)-1\right)+1=\frac{116}{125} \end{array}\right)
